src/named/PfCoreDefs.v
@@ -1,0 +1,429 @@
+Require Import mathcomp.ssreflect.all_ssreflect.
+Set Implicit Arguments.
+Unset Strict Implicit.
+Unset Printing Implicit Defensive.
+Set Bullet Behavior "Strict Subproofs".
+
+From Utils Require Import Utils.
+From Named Require Import Pf.
+
+Require Import String.
+
+
+Create HintDb pfcore discriminated.
+
+
+(* Denotes when a proof represents
+     an expression (as opposed to a relation
+     between 2 expressions)
+ *)
+Inductive is_exp : pf -> Prop :=
+| var_is_exp x : is_exp (pvar x)
+| con_is_exp name s
+  : List.Forall is_exp s ->
+    is_exp (pcon name s)
+| conv_is_exp pt p
+  : is_exp p ->
+    is_exp (conv pt p).
+Hint Constructors is_exp : pfcore.
+
+Fixpoint check_is_exp e : bool :=
+  match e with
+  | pvar _ => true
+  | pcon _ s => List.forallb check_is_exp s
+  | conv _ p => check_is_exp p
+  | _ => false
+  end.
+  
+Section TermsAndRules.
+  Context (l : pf_lang).
+
+  Inductive is_dom : pf -> pf -> Prop :=
+  | dom_var x : is_dom (pvar x) (pvar x)
+  | dom_con n pl pl_l
+    : List.Forall2 is_dom pl pl_l ->
+      is_dom (pcon n pl) (pcon n pl_l)
+  | dom_ax_sort n pl pl_l c p' p_r
+    : List.Forall2 is_dom pl pl_l ->
+      (n, sort_le_pf c p' p_r) \in l ->
+      is_dom (ax n pl) (pf_subst (with_names_from c pl_l) p')
+  | dom_ax_term n pl pl_l c p' p_r t
+    : List.Forall2 is_dom pl pl_l ->
+      (n, term_le_pf c p' p_r t) \in l ->
+      is_dom (ax n pl) (pf_subst (with_names_from c pl_l) p')
+  | dom_sym p p_r
+    : is_codom p p_r ->
+      is_dom (sym p) p_r
+  | dom_trans p1 p2 p1_l
+    : is_dom p1 p1_l ->
+      is_dom (trans p1 p2) p1_l
+  | dom_conv pt p p_l
+    : is_dom p p_l ->
+      is_dom (conv pt p) (conv pt p_l)
+  with is_codom : pf -> pf -> Prop :=
+  | codom_var x : is_codom (pvar x) (pvar x)
+  | codom_con n pl pl_r
+    : List.Forall2 is_codom pl pl_r ->
+      is_codom (pcon n pl) (pcon n pl_r)
+  | codom_ax_sort n pl pl_r c p' p_l
+    : List.Forall2 is_codom pl pl_r ->
+      (n, sort_le_pf c p_l p') \in l ->
+      is_codom (ax n pl) (pf_subst (with_names_from c pl_r) p')
+  | codom_ax_term n pl pl_r c p' p_l t
+    : List.Forall2 is_codom pl pl_r ->
+      (n, term_le_pf c p_l p' t) \in l ->
+      is_codom (ax n pl) (pf_subst (with_names_from c pl_r) p')
+  | codom_sym p p_r
+    : is_dom p p_r ->
+      is_codom (sym p) p_r
+  | codom_trans p1 p2 p2_r
+    : is_codom p2 p2_r ->
+      is_codom (trans p1 p2) p2_r
+  | codom_conv pt p p_r
+    : is_codom p p_r ->
+      is_codom (conv pt p) (conv pt p_r).
+  Hint Constructors is_dom is_codom : pfcore.
+
+      
+  (*TODO: move to OptionMonad *)
+  (*TODO: unused here*)
+  Import OptionMonad.
+  Fixpoint Mmap {A B} (f : A -> option B) (l_a : list A) : option (list B) :=
+    match l_a with
+    | [::] => do ret [::]
+    | a::l_a' =>
+      do l_b' <- Mmap f l_a';
+         b <- f a;
+         ret (b::l_b')
+    end.              
+
+  Section DomInnerLoop.
+    (*For some reason I need two copies of Mmap
+      for the mutual recursion to go through below.
+     *)
+    Context (dom : pf -> option pf)
+            (codom : pf -> option pf).
+    Fixpoint dom_args (pl : list pf) :=
+      match pl with
+      | [::] => do ret [::]
+      | a::pl' =>
+        do pl'_dom <- dom_args pl';
+           b <- dom a;
+           ret (b::pl'_dom)
+      end.
+
+    Fixpoint codom_args (pl : list pf) :=
+         match pl with
+         | [::] => do ret [::]
+         | a::pl' =>
+           do pl'_codom <- codom_args pl';
+              b <- codom a;
+              ret (b::pl'_codom)
+         end.
+  End DomInnerLoop.
+    
+  (*Pressupposition: p is ok and l is ok *)
+  Fixpoint dom (p:pf) :=
+    match p with
+    | pvar x => do ret (pvar x)
+    | pcon name pl => omap (pcon name) (dom_args dom pl)
+    | ax name pl =>
+      match named_list_lookup_err l name with
+      | Some (sort_le_pf c p' _)
+      | Some (term_le_pf c p' _ _) =>
+        do pl' <- dom_args dom pl;
+        ret pf_subst (with_names_from c pl') p'
+      | _ => None
+      end
+    | sym p => codom p
+    | trans p1 p2 => dom p1
+    | conv pt p' => omap (conv pt) (dom p')
+    end               
+ (*Pressupposition: p is ok and l is ok *)
+  with codom (p:pf) :=
+    match p with
+    | pvar x => do ret (pvar x)
+    | pcon name pl => omap (pcon name) (codom_args codom pl)
+    | ax name pl =>
+      match named_list_lookup_err l name with
+      | Some (sort_le_pf c _ p')
+      | Some (term_le_pf c _ p' _) =>
+        do pl' <- codom_args codom pl;
+        ret pf_subst (with_names_from c pl') p'
+      | _ => None
+      end
+    | sym p => dom p
+    | trans p1 p2 => codom p2
+    | conv pt p' => omap (conv pt) (codom p')
+    end.
+  
+  (*
+    Judgments for checking proofs of relations between programs.
+    Can check wfness of a program by identifying it with its
+    identity relation.
+
+    All assume lang_ok.
+    All ctxs (other than in ctx_ok) are assumed to satisfy ctx_ok.
+    Judgments whose assumptions take ctxs must ensure they are ok.
+    Sorts are not assumed to be ok; the term judgments should guarantee
+    that their sorts are ok and is_exp.
+   *)
+  
+  Inductive sort_ok : pf_ctx -> pf -> Prop :=
+  | sort_ok_ax : forall c c' name t1 t2 s,
+      (name, sort_le_pf c' t1 t2) \in l ->
+      args_ok c s c' ->
+      sort_ok c (ax name s)
+  | sort_ok_con : forall c name c' args s,
+      (name, (sort_rule_pf c' args)) \in l ->
+      args_ok c s c' ->
+      sort_ok c (pcon name s)
+  | sort_ok_trans : forall c t1 t t2,
+      sort_ok c t1 ->
+      sort_ok c t2 ->
+      is_codom t1 t ->
+      is_dom t2 t ->
+      sort_ok c (trans t1 t2)
+  | sort_ok_sym : forall c t, sort_ok c t -> sort_ok c (sym t)
+  with term_ok : pf_ctx -> pf -> pf -> Prop :=
+  | term_ok_ax : forall c c' name e1 e2 t s t',
+      (name, term_le_pf c' e1 e2 t) \in l ->
+      args_ok c s c' ->
+      (*non-obvious fact: the sort may not be a wfness proof if we don't project;
+        may be a non-identity relation due to s
+       *)
+      is_dom (pf_subst (with_names_from c' s) t) t' ->
+      term_ok c (ax name s) t'
+  | term_ok_con : forall c name c' args t t' s,
+      (name, (term_rule_pf c' args t)) \in l ->
+      args_ok c s c' ->
+      is_dom (pf_subst (with_names_from c' s) t) t' ->
+      (* same as above *)
+      term_ok c (pcon name s) t'
+  | term_ok_trans : forall c e1 e e2 t,
+      term_ok c e1 t ->
+      term_ok c e2 t ->
+      is_codom e1 e ->
+      is_dom e2 e ->
+      term_ok c (trans e1 e2) t
+  | term_ok_sym : forall c e t, term_ok c e t -> term_ok c (sym e) t
+  | term_ok_var : forall c x t,
+      (x,t) \in c ->
+      term_ok c (pvar x) t
+  (* Conversion:
+
+c |- e1 = e2 : t = t'
+                 ||
+c |- e1 = e2 : t' = t''
+
+   *)
+  | term_ok_conv : forall c e t tp t',
+      sort_ok c tp ->
+      term_ok c e t ->
+      is_dom tp t ->
+      is_codom tp t' ->
+      term_ok c (conv tp e) t'
+  with args_ok : pf_ctx -> list pf -> pf_ctx -> Prop :=
+  | args_ok_nil : forall c, args_ok c [::] [::]
+  | args_ok_cons : forall c s c' name e t t',
+      args_ok c s c' ->
+      (* assumed because the output ctx is wf: fresh name c' ->*)
+      is_dom (pf_subst (with_names_from c' s) t) t' ->
+      term_ok c e t' ->
+      args_ok c (e::s) ((name, t)::c').
+  
+  Inductive subst_ok : pf_ctx -> named_list pf -> pf_ctx -> Prop :=
+  | subst_ok_nil : forall c, subst_ok c [::] [::]
+  | subst_ok_cons : forall c s c' name e t t',
+      subst_ok c s c' ->
+      (* assumed because the output ctx is wf: fresh name c' ->*)
+      is_dom (pf_subst s t) t' ->
+      term_ok c e t' ->
+      subst_ok c ((name,e)::s) ((name, t)::c').
+
+  Inductive ctx_ok : pf_ctx -> Prop :=
+  | ctx_ok_nil : ctx_ok [::]
+  | ctx_ok_cons : forall name c v,
+      fresh name c ->
+      ctx_ok c ->
+      sort_ok c v ->
+      ctx_ok ((name,v)::c).
+
+  Variant rule_ok : rule_pf -> Prop :=
+  | sort_rule_ok : forall c args,
+      ctx_ok c ->
+      subseq args (map fst c) ->
+      rule_ok (sort_rule_pf c args)
+  | term_rule_ok : forall c args t,
+      ctx_ok c ->
+      sort_ok c t ->
+      subseq args (map fst c) ->
+      rule_ok (term_rule_pf c args t)
+  | sort_le_ok : forall c t1 t2,
+      ctx_ok c ->
+      is_exp t1 ->
+      is_exp t2 ->
+      sort_ok c t1 ->
+      sort_ok c t2 ->
+      rule_ok (sort_le_pf c t1 t2)
+  | term_le_ok : forall c e1 e2 t,
+      ctx_ok c ->
+      is_exp e1 ->
+      is_exp e2 ->
+      is_exp t ->
+      sort_ok c t ->
+      term_ok c e1 t ->
+      term_ok c e2 t ->
+      rule_ok (term_le_pf c e1 e2 t).
+
+  Hint Constructors sort_ok term_ok subst_ok args_ok ctx_ok rule_ok : pfcore.
+  
+  Section InnerLoop.
+    Context (check_term_ok : pf -> pf -> bool).
+
+    Fixpoint check_args_ok' (pl : list pf) (c' : pf_ctx) {struct pl} : bool :=
+      match pl, c' with
+      | [::], [::] => true
+      | p::pl', (_,t)::c'' =>
+        (check_term_ok p (pf_subst (with_names_from c'' pl') t)) &&
+        (check_args_ok' pl' c'')
+      |_,_=> false
+    end.
+
+    Fixpoint check_sort_ok' (pt : pf) : bool :=
+      match pt with
+      | pcon name pl =>
+        match named_list_lookup_err l name with
+        | Some (sort_rule_pf c' _) => check_args_ok' pl c'
+        | _ => false
+        end
+      | ax name pl =>
+        match named_list_lookup_err l name with
+        | Some (sort_le_pf c' _ _) => check_args_ok' pl c'
+        | _ => false
+        end
+      | sym p => check_sort_ok' p
+      | trans p1 p2 =>
+        (check_sort_ok' p1) &&
+        (check_sort_ok' p2) &&
+        (*TODO: will need to show that they are not none when the sorts are okay
+          because I am using the ==, but it reads more nicely this way
+         *)
+        (codom p1 == dom p2) 
+      | conv _ _ => false
+      | pvar _ => false
+      end.
+         
+  End InnerLoop.
+  
+  Fixpoint synth_term_ok (c : pf_ctx) e {struct e} : option pf :=
+    let check_term_ok e t := synth_term_ok c e == Some t in 
+    match e with
+    | pvar x => named_list_lookup_err c x
+    | pcon name pl =>
+      do (term_rule_pf c' _ t') <- named_list_lookup_err l name;
+         ! check_args_ok' check_term_ok pl c';
+         d <-(codom (pf_subst (with_names_from c' pl) t'));
+         ret d
+    | ax name pl =>
+      do (term_le_pf c' _ _ t') <- named_list_lookup_err l name;
+         ! check_args_ok' check_term_ok pl c';
+         d <-(codom (pf_subst (with_names_from c' pl) t'));
+         ret d
+    | sym p => synth_term_ok c p
+    | trans p1 p2 =>
+      do t1 <- synth_term_ok c p1;
+         t2 <- synth_term_ok c p2;
+         ! codom p1 == dom p2;
+         ! t1 == t2;
+         ret t2
+    | conv pt p' =>
+      do t1 <- synth_term_ok c p';
+         ! check_sort_ok' check_term_ok pt;
+         d <- dom pt;
+         ! t1 == d;
+         cd <- codom pt;
+         ret cd
+  end.
+
+  Definition check_term_ok c e t := synth_term_ok c e == Some t.
+  Definition check_sort_ok c p := check_sort_ok' (check_term_ok c) p.
+  Definition check_args_ok c pl c' := check_args_ok' (check_term_ok c) pl c'.
+
+  Fixpoint check_ctx_ok c :=
+    match c with
+    | [::] => true
+    | (name,t)::c' =>
+      (fresh name c') &&
+      (check_sort_ok c' t) &&
+      (check_ctx_ok c')
+    end.
+
+    
+  Definition check_rule_ok r :=
+    match r with
+    | sort_rule_pf c args =>
+      (check_ctx_ok c) && (subseq args (map fst c))
+    | term_rule_pf c args t =>
+      (check_ctx_ok c) &&
+      (subseq args (map fst c)) &&
+      (check_sort_ok c t)
+    | sort_le_pf c t1 t2 =>
+      (check_ctx_ok c) &&
+      (check_is_exp t1) &&
+      (check_is_exp t2) &&
+      (check_sort_ok c t1) &&
+      (check_sort_ok c t2)
+    | term_le_pf c e1 e2 t =>
+      (check_ctx_ok c) &&
+      (check_is_exp e1) &&
+      (check_is_exp e2) &&
+      (check_is_exp t) &&
+      (check_term_ok c e1 t) &&
+      (check_term_ok c e2 t) &&
+      (check_sort_ok c t)
+    end.
+  
+End TermsAndRules.
+
+Inductive lang_ok : pf_lang -> Prop :=
+| lang_ok_nil : lang_ok [::]
+| lang_ok_cons : forall name l r,
+    fresh name l ->
+    lang_ok l ->
+    rule_ok l r ->
+    lang_ok ((name,r)::l).
+
+
+Fixpoint check_lang_ok l :=
+    match l with
+    | [::] => true
+    | (name,r)::l' =>
+      (fresh name l') &&
+      (check_rule_ok l' r) &&
+      (check_lang_ok l')
+    end.
+
+(*TODO: move to Pf*)
+
+Inductive ws_pf {c : list string} : pf -> Prop :=
+| ws_var x : x \in c -> ws_pf (pvar x)
+| ws_con n l : List.Forall ws_pf l -> ws_pf (pcon n l)
+| ws_ax n l : List.Forall ws_pf l -> ws_pf (ax n l)
+| ws_sym p : ws_pf p -> ws_pf (sym p)
+| ws_trans p1 p2 : ws_pf p1 -> ws_pf p2 -> ws_pf (trans p1 p2)
+| ws_conv p1 p2 : ws_pf p1 -> ws_pf p2 -> ws_pf (conv p1 p2).
+
+Arguments ws_pf : clear implicits.
+
+
+(*TODO: move to Pf*)
+Fixpoint fv (p : pf) :=
+  match p with
+  | pvar x => [:: x]
+  | pcon _ l => flat_map fv l
+  | ax _ l => flat_map fv l
+  | sym p => fv p
+  | trans p1 p2 => fv p1 ++ fv p2
+  | conv p1 p2 => fv p1 ++ fv p2
+  end.
